CBPV/Lazy.lean
@@ -1,0 +1,219 @@
+import CBPV.CBN
+
+open Nat
+
+/-*-----------------
+  Lazy translation
+-----------------*-/
+
+/-* Translation of types *-/
+section
+set_option hygiene false
+local notation:40 "⟦" A:41 "⟧ᴸ" => transLazy A
+@[simp]
+def CBN.SType.transLazy : CBN.SType → ComType
+  | .Unit => .F .Unit
+  | .Sum A₁ A₂ => .F (.Sum (.U (⟦ A₁ ⟧ᴸ)) (.U (⟦ A₂ ⟧ᴸ)))
+  | .Prod B₁ B₂ => .F (.Pair (.U (⟦ B₁ ⟧ᴸ)) (.U (⟦ B₂ ⟧ᴸ)))
+  | .Arr A B => .F (.U (.Arr (.U (⟦ A ⟧ᴸ)) (⟦ B ⟧ᴸ)))
+end
+notation:40 "⟦" A:41 "⟧ᴸ" => CBN.SType.transLazy A
+
+theorem transF (B : CBN.SType) : ∃ A, (⟦ B ⟧ᴸ) = .F A := by
+  cases B <;> simp
+
+/-* Translation of contexts *-/
+section
+set_option hygiene false
+local notation:40 "⟦" Γ:41 "⟧ᴸ" => transLazy Γ
+@[simp]
+def CBN.Ctxt.transLazy : CBN.Ctxt → _root_.Ctxt
+  | .nil => .nil
+  | .cons Γ A => .cons (⟦ Γ ⟧ᴸ) (.U (⟦ A ⟧ᴸ))
+end
+notation:40 "⟦" Γ:41 "⟧ᴸ" => CBN.Ctxt.transLazy Γ
+
+/-* Translation of terms *-/
+section
+set_option hygiene false
+local notation:40 "⟦" t:41 "⟧ᴸ" => transLazy t
+@[simp]
+def CBN.Term.transLazy : CBN.Term → Com
+  | .var s => .force (.var s)
+  | .unit => .ret .unit
+  | .lam t => .ret (.thunk (.lam (⟦ t ⟧ᴸ)))
+  | .app t u =>
+    .letin (⟦ t ⟧ᴸ)
+      (.app (.force (.var 0)) (.thunk (renameCom succ (⟦ u ⟧ᴸ))))
+  | .inl t => .ret (.inl (.thunk (⟦ t ⟧ᴸ)))
+  | .inr t => .ret (.inr (.thunk (⟦ t ⟧ᴸ)))
+  | .case s t u =>
+    .letin (⟦ s ⟧ᴸ)
+      (.case (.var 0)
+        (renameCom (lift succ) (⟦ t ⟧ᴸ))
+        (renameCom (lift succ) (⟦ u ⟧ᴸ)))
+  | .prod t u => .ret (.pair (.thunk (⟦ t ⟧ᴸ)) (.thunk (⟦ u ⟧ᴸ)))
+  | .fst t => .letin (⟦ t ⟧ᴸ) (.unpair (.var 0) (.force (.var 1)))
+  | .snd t => .letin (⟦ t ⟧ᴸ) (.unpair (.var 0) (.force (.var 0)))
+  | .letin t u =>
+    .letin (⟦ t ⟧ᴸ)
+      (.letin (.ret (.thunk (.ret (.var 0))))
+        (renameCom (lift succ) (⟦ u ⟧ᴸ)))
+end
+notation:40 "⟦" t:41 "⟧ᴸ" => CBN.Term.transLazy t
+
+/-* Translation of stacks *-/
+section
+set_option hygiene false
+local notation:40 "⟦" k:41 "⟧ᴸ" => transLazy k
+@[simp]
+def CBN.K.transLazy : CBN.K → CK.K
+  | [] => []
+  | .app u :: k   => .letin (.app (.force (.var 0))
+                        (.thunk (renameCom succ (⟦ u ⟧ᴸ)))) :: (⟦ k ⟧ᴸ)
+  | .case t u :: k => .letin (.case (.var 0)
+                        (renameCom (lift succ) (⟦ t ⟧ᴸ))
+                        (renameCom (lift succ) (⟦ u ⟧ᴸ))) :: (⟦ k ⟧ᴸ)
+  | .fst :: k => .letin (.unpair (.var 0) (.force (.var 1))) :: (⟦ k ⟧ᴸ)
+  | .snd :: k => .letin (.unpair (.var 0) (.force (.var 0))) :: (⟦ k ⟧ᴸ)
+  | .letin u :: k => .letin
+                        (.letin (.ret (.thunk (.ret (.var 0))))
+                          (renameCom (lift succ) (⟦ u ⟧ᴸ))) :: (⟦ k ⟧ᴸ)
+end
+notation:40 "⟦" k:41 "⟧ᴸ" => CBN.K.transLazy k
+
+/-* Translation of terms with arbitrary π-expansion *-/
+section
+set_option hygiene false
+local infix:40 "↦ₗ" => expandLazy
+inductive CBN.Term.expandLazy : CBN.Term → Com → Prop where
+  | var {s} : .var s ↦ₗ .force (.var s)
+  | unit : .unit ↦ₗ .ret .unit
+  | lam {t m} : t ↦ₗ m → .lam t ↦ₗ .ret (.thunk (.lam m))
+  | app {t u m n} : t ↦ₗ m → u ↦ₗ n →
+    .app t u ↦ₗ
+      .letin m
+        (.app (.force (.var 0)) (.thunk (renameCom succ n)))
+  | inl {t m} : t ↦ₗ m → .inl t ↦ₗ .ret (.inl (.thunk m))
+  | inr {t m} : t ↦ₗ m → .inr t ↦ₗ .ret (.inr (.thunk m))
+  | case {s t u ms mt mu} : s ↦ₗ ms → t ↦ₗ mt → u ↦ₗ mu →
+    .case s t u ↦ₗ
+      .letin ms
+        (.case (.var 0)
+          (renameCom (lift succ) mt)
+          (renameCom (lift succ) mu))
+  | prod {t u m n} : t ↦ₗ m → u ↦ₗ n →
+    .prod t u ↦ₗ .ret (.pair (.thunk m) (.thunk n))
+  | fst {t m} : t ↦ₗ m →
+    .fst t ↦ₗ .letin m (.unpair (.var 0) (.force (.var 1)))
+  | snd {t m} : t ↦ₗ m →
+    .snd t ↦ₗ .letin m (.unpair (.var 0) (.force (.var 0)))
+  | letin {t u m n} : t ↦ₗ m → u ↦ₗ n →
+    .letin t u ↦ₗ
+      .letin m
+        (.letin (.ret (.thunk (.ret (.var 0))))
+          (renameCom (lift succ) n))
+  | ft {t m} : t ↦ₗ m → t ↦ₗ .force (.thunk m)
+end
+infix:40 "↦ₗ" => CBN.Term.expandLazy
+
+/-*---------------------------------------
+  Preservation properties of translation
+---------------------------------------*-/
+
+namespace Lazy
+
+theorem transExpand {t} : t ↦ₗ (⟦ t ⟧ᴸ) := by
+  induction t <;> constructor <;> assumption
+
+/-* Translation is type preserving *-/
+
+theorem presIn {x A Γ} (h : CBN.In x A Γ) : (⟦ Γ ⟧ᴸ) ∋ x ∶ .U (⟦ A ⟧ᴸ) := by
+  induction h <;> constructor; assumption
+
+theorem preservation {Γ t A} (h : Γ ⊢ₛ t ∶ A) : (⟦ Γ ⟧ᴸ) ⊢ (⟦ t ⟧ᴸ) ∶ (⟦ A ⟧ᴸ) := by
+  induction h
+  case var mem => exact .force (.var (presIn mem))
+  case unit => exact .ret .unit
+  case lam ih => exact .ret (.thunk (.lam ih))
+  case app iht ihu => exact .letin iht (.app (.force (.var .here)) (.thunk (wtWeakenCom ihu)))
+  case inl ih => exact .ret (.inl (.thunk ih))
+  case inr ih => exact .ret (.inr (.thunk ih))
+  case case ihs iht ihu => exact .letin ihs (.case (.var .here) (wtWeakenCom₂ iht) (wtWeakenCom₂ ihu))
+  case prod iht ihu => exact .ret (.pair (.thunk iht) (.thunk ihu))
+  case fst ih => exact .letin ih (.unpair (.var .here) (.force (.var (.there .here))))
+  case snd ih => exact .letin ih (.unpair (.var .here) (.force (.var .here)))
+  case letin B₁ _ _ _ iht ihu =>
+    let ⟨A, e⟩ := transF B₁
+    simp at ihu; rw [e] at iht ihu
+    exact .letin iht (.letin (.ret (.thunk (.ret (.var .here)))) (wtWeakenCom₂ ihu))
+
+/-* Translation commutes with renaming and substitution *-/
+
+theorem expandRename {ξ t m} (h : t ↦ₗ m) : CBN.rename ξ t ↦ₗ renameCom ξ m := by
+  induction h generalizing ξ
+  all_goals try simp [← renameLiftRenameCom, renameLiftLiftRename]
+  all_goals constructor <;> apply_assumption
+
+theorem expandUp {σ : Nat → CBN.Term} {σ' : Nat → Val}
+  (h : ∀ x, σ x ↦ₗ .force (σ' x)) : ∀ x, (⇑ σ) x ↦ₗ .force ((⇑ σ') x) := by
+  have e {ξ v} : .force (renameVal ξ v) = renameCom ξ (.force v) := rfl
+  intro n; cases n
+  case zero => exact .var
+  case succ n => simp [up]; rw [e]; exact expandRename (h n)
+
+theorem expandSubst {σ σ' t} (h : ∀ x, σ x ↦ₗ .force (σ' x)) : CBN.subst σ t ↦ₗ substCom σ' (⟦t⟧ᴸ) := by
+  induction t generalizing σ σ'
+  all_goals try simp [← renameUpSubstCom, ← renameUpLiftSubst]
+  case var => exact h _
+  all_goals constructor <;> apply_rules [expandUp]
+
+theorem expandSubstSingle {t u} : CBN.subst (u +: .var) t ↦ₗ (⟦t⟧ᴸ) ⦃ Val.thunk (⟦ u ⟧ᴸ) +: .var ⦄ := by
+  refine expandSubst (λ n ↦ ?_); cases n <;> constructor; simp; exact transExpand
+
+theorem simulation {t u k k'} (r : ⟨t, k⟩ ⤳ₙ ⟨u, k'⟩) : ∃ m, ⟨⟦ t ⟧ᴸ, ⟦ k ⟧ᴸ⟩ ⤳⋆ ⟨m, ⟦ k' ⟧ᴸ⟩ ∧ u ↦ₗ m := by
+  generalize et : (t, k)  = ck  at r
+  generalize eu : (u, k') = ck' at r
+  induction r
+  all_goals injection et with et ek; subst et ek
+  all_goals injection eu with eu ek; subst eu ek
+  case β t u =>
+    refine ⟨⟦ t ⟧ᴸ ⦃ .thunk (⟦ u ⟧ᴸ) ⦄, ?_, expandSubstSingle⟩
+    calc
+      _ ⤳ _ := .ζ
+      _ ⤳ _ := by exact .app
+      _ ⤳ _ := .μ
+      _ ⤳ _ := .β
+      _ = _ := by simp; rw [← substDropCom]
+  case ιl s t _ =>
+    refine ⟨⟦ t ⟧ᴸ ⦃ .thunk (⟦ s ⟧ᴸ)⦄, ?_, expandSubstSingle⟩
+    calc
+      _ ⤳ _ := .ζ
+      _ ⤳ _ := by exact .ιl
+      _ = _ := by rw [← substUnion, substDropCom₂]
+  case ιr s _ u =>
+    refine ⟨⟦ u ⟧ᴸ ⦃ .thunk (⟦ s ⟧ᴸ)⦄, ?_, expandSubstSingle⟩
+    calc
+      _ ⤳ _ := .ζ
+      _ ⤳ _ := by exact .ιr
+      _ = _ := by rw [← substUnion, substDropCom₂]
+  case π1 | π2 =>
+    refine ⟨_, ?_, transExpand⟩
+    calc
+      _ ⤳ _ := .ζ
+      _ ⤳ _ := by exact .π
+      _ ⤳ _ := by exact .μ
+  case ζlam | ζinl | ζinr | ζprod =>
+    refine ⟨_, ?_, expandSubstSingle⟩
+    calc
+      _ ⤳ _ := .ζ
+      _ ⤳ _ := by exact .letin
+      _ ⤳ _ := .ζ
+      _ = _ := by simp [← substUnion, substDropCom₂]
+  case app => exact ⟨_, .once .letin, transExpand⟩
+  case case => exact ⟨_, .once .letin, transExpand⟩
+  case fst => exact ⟨_, .once .letin, transExpand⟩
+  case snd => exact ⟨_, .once .letin, transExpand⟩
+  case letin! => exact ⟨_, .once .letin, transExpand⟩
+
+end Lazy
